support for standalone comments

src/InputAst.ml
@@ -100,6 +100,7 @@ and expr =
   | EBufCreateNoInit of (lifetime * expr)
   | EAbortT of (string * typ)
   | EComment of (string * expr * string)
+  | EStandaloneComment of string
 
 and branches =
   branch list
