src/InputAstToAst.ml
@@ -183,6 +183,8 @@ and mk_expr = function
       mk (EFun (mk_binders bs, mk_expr e, mk_typ t))
   | I.EComment (before, e, after) ->
       mk (EComment (before, mk_expr e, after))
+  | I.EStandaloneComment s ->
+      mk (EStandaloneComment s)
 
 and mk_branches branches =
   List.map mk_branch branches
